process/InitMem.v
@@ -1,0 +1,208 @@
+Require Import Maps Coqlib Integers List.
+Require Import AST Globalenvs Memory Values.
+Import ListNotations.
+
+Section INIT_MEM.
+  Context (se: Genv.symtbl).
+
+  Program Definition empty : mem :=
+    Mem.mkmem (PMap.init (ZMap.init Undef))
+      (PMap.init (fun ofs k => None))
+      (Genv.genv_next se) true _ _ _.
+
+  (* like [Mem.alloc], but only changes the perm *)
+  Program Definition init_perm (m: mem) (b: block) (lo hi: Z) :=
+    if plt b m.(Mem.nextblock) then
+      Some
+        (Mem.mkmem
+           m.(Mem.mem_contents)
+           (PMap.set b
+              (fun ofs k => if zle lo ofs && zlt ofs hi then Some Freeable else None)
+              m.(Mem.mem_access))
+           m.(Mem.nextblock) m.(Mem.alloc_flag) _ _ _)
+    else None.
+  Next Obligation.
+    repeat rewrite PMap.gsspec. destruct (peq b0 b).
+    - subst b. destruct (zle lo ofs && zlt ofs hi); red; auto with mem.
+    - apply Mem.access_max.
+  Qed.
+  Next Obligation.
+    repeat rewrite PMap.gsspec. destruct (peq b0 b).
+    - subst b. elim H0. exact H.
+    - eapply Mem.nextblock_noaccess. exact H0.
+  Qed.
+  Next Obligation. apply Mem.contents_default. Qed.
+
+  Definition init_global' (m: mem) (b: block) (g: globdef unit unit): option mem :=
+    match g with
+    | Gfun f =>
+        match init_perm m b 0 1 with
+        | Some m1 => Mem.drop_perm m1 b 0 1 Nonempty
+        | None => None
+        end
+    | Gvar v =>
+        let init := v.(gvar_init) in
+        let sz := init_data_list_size init in
+        match init_perm m b 0 sz with
+        | Some m1 =>
+            match store_zeros m1 b 0 sz with
+            | None => None
+            | Some m2 =>
+                match Genv.store_init_data_list se m2 b 0 init with
+                | None => None
+                | Some m3 => Mem.drop_perm m3 b 0 sz (Genv.perm_globvar v)
+                end
+            end
+        | None => None
+        end
+    end.
+
+  Definition init_global (m: mem) (idg: ident * globdef unit unit): option mem :=
+    match idg with
+    | (id, g) =>
+        match Genv.find_symbol se id with
+        | Some b => init_global' m b g
+        | None => None
+        end
+    end.
+
+  Fixpoint init_globals (m: mem) (gl: list (ident * globdef unit unit)): option mem :=
+    match gl with
+    | [] => Some m
+    | g :: gl' =>
+        match init_global m g with
+        | None => None
+        | Some m' => init_globals m' gl'
+        end
+    end.
+
+  Definition init_mem (p: AST.program unit unit) : option mem :=
+    init_globals empty p.(AST.prog_defs).
+
+  Lemma init_perm_inv m1 m2 lo hi b:
+    init_perm m1 b lo hi = Some m2 ->
+    forall ofs k, lo <= ofs < hi -> Mem.perm m2 b ofs k Freeable.
+  Proof.
+    intros. unfold init_perm in H. destruct plt; inv H.
+    unfold Mem.perm. cbn. rewrite PMap.gss.
+    destruct (zle lo ofs && zlt ofs hi) eqn: H1; try constructor.
+    exfalso. destruct zle eqn: H2; try lia. destruct zlt eqn: H3; try lia.
+    cbn in H1. congruence.
+  Qed.
+
+  Lemma init_global_exists:
+    forall m idg,
+      (exists b, Genv.find_symbol se (fst idg) = Some b /\
+              Plt b m.(Mem.nextblock)) ->
+      match idg with
+      | (id, Gfun f) => True
+      | (id, Gvar v) =>
+          Genv.init_data_list_aligned 0 v.(gvar_init)
+          /\ forall i o, In (Init_addrof i o) v.(gvar_init) -> exists b, Genv.find_symbol se i = Some b
+      end ->
+      exists m', init_global m idg = Some m'.
+  Proof.
+    intros m [id [f|v]] [b [Hb1 Hb2]]; intros; simpl in *; rewrite Hb1.
+    - destruct (init_perm m b 0 1) as [m1|] eqn:H1.
+      2: { exfalso. unfold init_perm in H1. destruct plt; [ inv H1 | contradiction ]. }
+      destruct (Mem.range_perm_drop_2 m1 b 0 1 Nonempty) as [m2 DROP].
+      red; intros; eapply init_perm_inv; eauto.
+      exists m2. eauto.
+    - destruct H as [P Q].
+      set (sz := init_data_list_size (gvar_init v)).
+      destruct (init_perm m b 0 sz) as [m1|] eqn:H1.
+      2: { exfalso. unfold init_perm in H1. destruct plt; [ inv H1 | contradiction ]. }
+      assert (P1: Mem.range_perm m1 b 0 sz Cur Freeable) by (red; intros; eapply init_perm_inv; eauto).
+      exploit (@Genv.store_zeros_exists m1 b 0 sz).
+      { red; intros. apply Mem.perm_implies with Freeable; auto with mem. }
+      intros [m2 ZEROS]. rewrite ZEROS.
+      assert (P2: Mem.range_perm m2 b 0 sz Cur Freeable).
+      { red; intros. erewrite <- Genv.store_zeros_perm by eauto. eauto. }
+      exploit (@Genv.store_init_data_list_exists se b (gvar_init v) m2 0); eauto.
+      { red; intros. apply Mem.perm_implies with Freeable; auto with mem. }
+      intros [m3 STORE]. rewrite STORE.
+      assert (P3: Mem.range_perm m3 b 0 sz Cur Freeable).
+      { red; intros. erewrite <- Genv.store_init_data_list_perm by eauto. eauto. }
+      destruct (Mem.range_perm_drop_2 m3 b 0 sz (Genv.perm_globvar v)) as [m4 DROP]; auto.
+      exists m4; auto.
+  Qed.
+
+  Lemma init_perm_nextblock m1 m2 b lo hi:
+    init_perm m1 b lo hi = Some m2 ->
+    Mem.nextblock m2 = Mem.nextblock m1.
+  Proof.
+    intros. unfold init_perm in H. destruct plt; inv H.
+    cbn. reflexivity.
+  Qed.
+
+  Lemma init_global_nextblock m1 m2 idg:
+    init_global m1 idg = Some m2 ->
+    Mem.nextblock m1 = Mem.nextblock m2.
+  Proof.
+    intros. unfold init_global in H. destruct idg as [id [f|v]]; simpl in H.
+    - destruct (Genv.find_symbol se id) as [b|] eqn: H1; inv H.
+      destruct (init_perm m1 b 0 1) as [m|] eqn: A1; inv H2.
+      erewrite <- init_perm_nextblock; [ | eauto ].
+      erewrite <- Mem.nextblock_drop; eauto.
+    - destruct (Genv.find_symbol se id) as [b|] eqn: H1; inv H.
+      destruct init_perm as [m3|] eqn: A1; inv H2.
+      destruct store_zeros as [m4|] eqn: A2; inv H0.
+      destruct Genv.store_init_data_list as [m5|] eqn: A3; inv H2.
+      erewrite <- init_perm_nextblock; [ | eauto ].
+      erewrite <- Genv.store_zeros_nextblock; [ | eauto ].
+      erewrite <- Genv.store_init_data_list_nextblock; [ | eauto ].
+      erewrite <- Mem.nextblock_drop; eauto.
+  Qed.
+
+  Lemma init_mem_exists p:
+    (forall id v, In (id, Gvar v) (AST.prog_defs p) ->
+             Genv.init_data_list_aligned 0 v.(gvar_init)
+             /\ forall i o, In (Init_addrof i o) v.(gvar_init) -> exists b, Genv.find_symbol se i = Some b) ->
+    Genv.valid_for p se ->
+    exists m, init_mem p = Some m.
+  Proof.
+    intros. unfold init_mem.
+    assert (H1: forall id g,
+               In (id, g) (AST.prog_defs p) ->
+               exists b, Genv.find_symbol se id = Some b
+                    /\ Plt b (Mem.nextblock empty)).
+    {
+      intros. edestruct prog_defmap_dom as [g' Hg'].
+      unfold prog_defs_names. apply in_map_iff.
+      exists (id, g). split; eauto. cbn in Hg'.
+      specialize (H0 _ _ Hg') as (b & ? & Hb & ? & ?).
+      exists b; split; eauto.
+      unfold empty. cbn. eapply Genv.genv_symb_range.
+      apply Hb.
+    }
+    clear H0.
+    revert H H1. generalize (AST.prog_defs p) empty.
+    induction l as [ | idg l ]; simpl; intros.
+    - exists m. reflexivity.
+    - destruct (@init_global_exists m idg) as [m1 A1].
+      + destruct idg as [id g]. apply (H1 id g). left; easy.
+      + destruct idg as [id [f|v]]; eauto.
+      + rewrite A1. edestruct (IHl m1) as [m2 IH]; eauto.
+        intros. erewrite <- init_global_nextblock; eauto.
+  Qed.
+
+  Lemma init_mem_nextblock p m:
+    init_mem p = Some m ->
+    Mem.nextblock m = Genv.genv_next se.
+  Proof.
+    assert (H: Mem.nextblock empty = Genv.genv_next se) by reflexivity.
+    revert H. unfold init_mem. generalize (AST.prog_defs p) empty.
+    induction l as [ | idg l ]; simpl; intros.
+    - inv H0. eauto.
+    - destruct init_global eqn: A1; inv H0.
+      erewrite <- IHl; [ eauto | | eauto ].
+      rewrite <- H. symmetry.  eapply init_global_nextblock; eauto.
+  Qed.
+
+  Lemma init_mem_alloc_flag p m:
+    init_mem p = Some m ->
+    Mem.alloc_flag m = true.
+  Proof.
+  Admitted.
+
+End INIT_MEM.
