process/Load.v
@@ -1,0 +1,393 @@
+Require Import Coqlib Integers.
+
+Require Import Events LanguageInterface Smallstep Globalenvs Values Memory.
+Require Import AST Ctypes Clight.
+Require Import Lifting Encapsulation.
+
+Require Import List Maps.
+Import ListNotations.
+Require Import Machregs Asm.
+
+Require Import InitMem With.
+
+Notation tint := (Tint I32 Unsigned noattr).
+
+Definition main_sig := signature_of_type Tnil tint cc_default.
+
+Section INIT_C.
+  Context (prog: Clight.program).
+  Let sk := erase_program prog.
+  Section WITH_SE.
+
+    Context (se: Genv.symtbl).
+    Let ge := Genv.globalenv se prog.
+    Inductive init_c_initial_state (q: query li_wp) : option int -> Prop :=
+    | init_c_initial_state_intro: init_c_initial_state q None.
+    Inductive init_c_at_external: option int -> query li_c -> Prop :=
+    | init_c_at_external_intro vf m f main b:
+      init_mem se sk = Some m ->
+      Genv.invert_symbol se b = Some main ->
+      vf = Vptr b Ptrofs.zero ->
+      prog_main prog = Some main ->
+      (prog_defmap prog) ! main = Some (Gfun f) ->
+      init_c_at_external None (cq vf main_sig [] m).
+    Inductive init_c_after_external: option int -> reply li_c -> option int -> Prop :=
+    | init_c_after_external_intro i m:
+      init_c_after_external None (cr (Vint i) m) (Some i).
+    Inductive init_c_final_state: option int -> reply li_wp -> Prop :=
+    | inic_c_final_state_intro i: init_c_final_state (Some i) i.
+
+  End WITH_SE.
+  Program Definition init_c: Smallstep.semantics li_c li_wp :=
+    {|
+      activate se :=
+        {|
+          Smallstep.step _ _ _ _ := False;
+          Smallstep.initial_state := init_c_initial_state;
+          Smallstep.at_external := init_c_at_external se;
+          Smallstep.after_external := init_c_after_external;
+          Smallstep.final_state := init_c_final_state;
+          Smallstep.globalenv := Genv.globalenv se prog;
+        |};
+      skel := sk;
+      footprint i := False
+    |}.
+End INIT_C.
+
+Section INIT_ASM.
+  Context (prog: program).
+  Let sk := erase_program prog.
+  Section WITH_SE.
+
+    Context (se: Genv.symtbl).
+    Let ge := Genv.globalenv se prog.
+    Inductive init_asm_initial_state (q: query li_wp) : option int -> Prop :=
+    | init_asm_initial_state_intro: init_asm_initial_state q None.
+    Inductive init_asm_at_external: option int -> query li_asm -> Prop :=
+    | init_asm_at_external_intro m rs f main vf b:
+      init_mem se sk = Some m ->
+      AST.prog_main prog = Some main ->
+      (prog_defmap prog) ! main = Some (Gfun f) ->
+      Genv.invert_symbol se b = Some main ->
+      vf = Vptr b Ptrofs.zero ->
+      (* (* TODO: use invert_symbol to associate main with a block *) *)
+      (* Genv.find_funct ge vf = Some f -> *)
+      (* [RSP] need to be qualified as Mach.valid_blockv, so it's using vf instead
+      of Vnullptr. See Mach.v for more details *)
+      rs = (((Pregmap.init Vundef) # PC <- vf) # RSP <- vf) # RA <- Vnullptr ->
+      init_asm_at_external None (rs, m).
+    Inductive init_asm_after_external: option int -> reply li_asm -> option int -> Prop :=
+    | init_asm_after_external_intro i rs m:
+      rs#(IR RAX) = Vint i ->
+      init_asm_after_external None (rs, m) (Some i).
+    Inductive init_asm_final_state: option int -> reply li_wp -> Prop :=
+    | inic_asm_final_state_intro i: init_asm_final_state (Some i) i.
+
+  End WITH_SE.
+  Program Definition init_asm: Smallstep.semantics li_asm li_wp :=
+    {|
+      activate se :=
+        {|
+          Smallstep.step _ _ _ _ := False;
+          Smallstep.initial_state := init_asm_initial_state;
+          Smallstep.at_external := init_asm_at_external se;
+          Smallstep.after_external := init_asm_after_external;
+          Smallstep.final_state := init_asm_final_state;
+          Smallstep.globalenv := Genv.globalenv se prog;
+        |};
+      skel := sk;
+      footprint i := False
+    |}.
+End INIT_ASM.
+
+Require Import Compiler.
+
+Section INIT_C_ASM.
+
+  Local Transparent Archi.ptr64.
+
+  Lemma init_c_asm p tp:
+    match_prog p tp -> forward_simulation cc_compcert 1 (init_c p) (init_asm tp).
+  Proof.
+    intros H. assert (Hsk: erase_program p = erase_program tp).
+    { apply clight_semantic_preservation in H as [H1 ?].
+      apply H1. }
+    constructor. econstructor. apply Hsk.
+    intros. reflexivity.
+    intros. instantiate (1 := fun _ _ _ => _). cbn beta. destruct H0.
+    eapply forward_simulation_step with (match_states := eq).
+    - intros. inv H0. inv H2.
+      eexists; split; eauto. constructor.
+    - intros. inv H2. exists r1. split; constructor.
+    - intros. inv H2.
+      eexists _, (_, m).
+      repeat apply conj.
+      + assert (exists tf, (prog_defmap tp) ! main = Some (Gfun tf)) as (tf & Htf).
+        { assert ((prog_defmap (erase_program p)) ! main = Some (Gfun tt)).
+          rewrite erase_program_defmap. unfold option_map. rewrite H7. reflexivity.
+          rewrite Hsk in H0. rewrite erase_program_defmap in H0.
+          unfold option_map in H0.
+          destruct (prog_defmap tp) ! main as [[tf|]|] eqn: Htf; inv H0.
+          exists tf. split; eauto. }
+        econstructor; eauto.
+        * rewrite <- Hsk. eauto.
+        * replace (AST.prog_main tp) with (AST.prog_main (erase_program tp))
+            by reflexivity.
+          rewrite <- Hsk. apply H6.
+      + unfold cc_compcert.
+        (* cklr *)
+        instantiate (1 := (se1, existT _ 0%nat _, _)).
+        exists (cq (Vptr b Ptrofs.zero) main_sig [] m). split.
+        { reflexivity. }
+        (* inv wt_c *)
+        instantiate (1 := (se1, (se1, main_sig), _)).
+        exists (cq (Vptr b Ptrofs.zero) main_sig [] m). split.
+        { repeat constructor. }
+        (* lessdef_c *)
+        instantiate (1 := (se1, tt, _)).
+        exists (cq (Vptr b Ptrofs.zero) main_sig [] m). split.
+        { repeat constructor. }
+        (* cc_c_locset *)
+        instantiate (1 := (se1, main_sig, _)).
+        eexists (Conventions.lq (Vptr b Ptrofs.zero) main_sig (CallConv.make_locset (Mach.Regmap.init Vundef) m (Vptr b Ptrofs.zero)) m). split.
+        { constructor. unfold Conventions1.loc_arguments. cbn.
+          destruct Archi.win64; reflexivity. }
+        (* cc_locset_mach *)
+        set (rs := ((((Pregmap.init Vundef) # PC <- (Vptr b Ptrofs.zero)) # SP <- (Vptr b Ptrofs.zero)) # RA <- Vnullptr)).
+        instantiate (1 := (se1, CallConv.lmw main_sig (Mach.Regmap.init Vundef) m (Vptr b Ptrofs.zero), _)).
+        eexists (Mach.mq rs#PC rs#SP rs#RA (Mach.Regmap.init Vundef) m). split.
+        { repeat constructor.
+          red. unfold Conventions.size_arguments. cbn. destruct Archi.win64; reflexivity. }
+        (* cc_mach_asm *)
+        instantiate (1 := (se1, ((((Pregmap.init Vundef) # PC <- (Vptr b Ptrofs.zero)) # RSP <- (Vptr b Ptrofs.zero)) # RA <- Vnullptr, Mem.nextblock m), _)).
+        eexists ((((Pregmap.init Vundef) # PC <- (Vptr b Ptrofs.zero)) # RSP <- (Vptr b Ptrofs.zero)) # RA <- Vnullptr, m). split.
+        { econstructor; cbn; try congruence.
+          - constructor. erewrite init_mem_nextblock; eauto.
+            apply Genv.invert_find_symbol in H4.
+            exploit @Genv.genv_symb_range; eauto.
+          - intros. destruct r; eauto. }
+        (* cc_asm vainj *)
+        instantiate (1 := (se1, Inject.injw (Mem.flat_inj (Mem.nextblock m)) (Mem.nextblock m) (Mem.nextblock m))).
+        repeat apply conj; cbn; eauto; try easy.
+        * intros. destruct r; eauto; cbn; try constructor.
+          eapply Val.inject_ptr. unfold Mem.flat_inj. admit. admit. admit.
+        * constructor; cbn.
+          -- erewrite init_mem_nextblock; eauto. reflexivity.
+          -- intros x Hx.  admit.
+          -- constructor. unfold Mem.inject.
+             (* Search (Mem.inject _ ?m ?m). *)
+             (* Search Mem.inject_neutral. *)
+             admit.
+      + cbn. repeat apply conj; eauto. constructor. eauto.
+        constructor; cbn.
+        (* Search (Genv.match_stbls _ ?se ?se). *)
+        admit. admit. admit.
+      + intros. inv H2. exists (Some i). split; eauto.
+        cbn in H0.
+        destruct H0 as (r3 & Hr3 & HR). inv Hr3.
+        destruct HR as (r3 & Hr3 & HR). inv Hr3.
+        destruct HR as (r3 & Hr3 & HR). inv Hr3. inv H9.
+        destruct HR as (r3 & Hr3 & HR). inv Hr3. cbn in H9.
+        destruct HR as (r3 & Hr3 & HR). inv Hr3.
+        specialize (H13 AX). rewrite <- H9 in H13.
+        exploit H13. cbn. left. reflexivity. intros HAX.
+        destruct HR as ((rs & mx) & Hr3 & Hr4). inv Hr3.
+        specialize (H20 AX). rewrite HAX in H20. cbn in H20.
+        destruct Hr4 as ((? & ?) & ? & Hr). destruct r2.
+        inv Hr. specialize (H5 RAX). rewrite <- H20 in H5.
+        destruct H2. cbn in H10. cbn in H5. inv H5.
+        constructor. easy.
+    - easy.
+    - easy.
+  Admitted.
+
+End INIT_C_ASM.
+
+Variant sys_query :=
+  | write_query: list byte -> sys_query
+  | read_query: int64 -> sys_query.
+
+Variant sys_reply :=
+  | write_reply: int -> sys_reply
+  | read_reply: list byte -> sys_reply.
+
+Definition li_sys :=
+  {|
+    query := sys_query;
+    reply := sys_reply;
+    entry q := Vundef;
+  |}.
+
+Notation tvoid := (Tvoid).
+Notation tchar := (Tint I8 Unsigned noattr).
+Notation tlong := (Tlong Unsigned noattr).
+Notation tptr := (fun ty => Tpointer ty noattr).
+
+Definition rw_parameters := Tcons tint (Tcons (tptr tchar) (Tcons tlong Tnil)).
+Definition rw_type :=
+  Tfunction rw_parameters tint cc_default.
+Definition rw_sig : signature :=
+  signature_of_type rw_parameters tvoid cc_default.
+Definition write : Clight.fundef :=
+  External (EF_external "write" rw_sig) rw_parameters tint cc_default.
+Definition read : Clight.fundef :=
+  External (EF_external "read" rw_sig) rw_parameters tint cc_default.
+
+Section SYS.
+  Context (prog: Clight.program).
+  Let sk := erase_program prog.
+  Section WITH_SE.
+    Context (se: Genv.symtbl).
+    Let ge := globalenv se prog.
+    Variant sys_state :=
+      | sys_read_query (n: int64) (b: block) (ofs: ptrofs) (m: mem)
+      | sys_read_reply (bytes: list byte) (b: block) (ofs: ptrofs) (m: mem)
+      | sys_write_query (bytes: list byte) (m: mem)
+      | sys_write_reply (n: int) (m: mem).
+
+    Inductive sys_c_initial_state: query li_c -> sys_state -> Prop :=
+    | sys_c_initial_state_read vf args m n b ofs:
+      Genv.find_funct ge vf = Some read ->
+      args = [ Vint (Int.repr 0); Vptr b ofs; Vlong n ] ->
+      sys_c_initial_state (cq vf rw_sig args m) (sys_read_query n b ofs m)
+    | sys_c_initial_state_write vf args m bytes bytes_val b ofs len:
+      Genv.find_funct ge vf = Some write ->
+      args = [ Vint (Int.repr 1); Vptr b ofs; Vlong (Int64.repr len) ] ->
+      Mem.loadbytes m b (Ptrofs.unsigned ofs) len = Some bytes_val ->
+      map Byte bytes = bytes_val ->
+      sys_c_initial_state (cq vf rw_sig args m) (sys_write_query bytes m).
+
+    Inductive sys_c_at_external: sys_state -> query (li_sys + li_sys) -> Prop :=
+    | sys_c_at_external_read n b ofs m:
+      sys_c_at_external (sys_read_query n b ofs m) (inl (read_query n))
+    | sys_c_at_external_write bytes m:
+      sys_c_at_external (sys_write_query bytes m) (inr (write_query bytes)).
+
+    Inductive sys_c_after_external: sys_state -> reply (li_sys + li_sys) -> sys_state -> Prop :=
+    | sys_c_after_external_read n b ofs m bytes:
+      Z.of_nat (length bytes) <= Int64.unsigned n ->
+      sys_c_after_external (sys_read_query n b ofs m) (inl (read_reply bytes)) (sys_read_reply bytes b ofs m)
+    | sys_c_after_external_write n m bytes:
+      sys_c_after_external (sys_write_query bytes m) (inr (write_reply n)) (sys_write_reply n m).
+
+    Inductive sys_c_final_state: sys_state -> reply li_c -> Prop :=
+    | sys_c_final_state_read bytes b ofs bytes_val m len m':
+      len = Z.of_nat (length bytes) ->
+      Mem.storebytes m b (Ptrofs.unsigned ofs) bytes_val = Some m' ->
+      map Byte bytes = bytes_val ->
+      sys_c_final_state (sys_read_reply bytes b ofs m) (cr (Vint (Int.repr len)) m')
+    | sys_c_final_state_write n m:
+      sys_c_final_state (sys_write_reply n m) (cr (Vint n) m).
+
+  End WITH_SE.
+  Definition sys_c: Smallstep.semantics (li_sys + li_sys) li_c :=
+    {|
+      activate se :=
+        {|
+          Smallstep.step _ _ _ _ := False;
+          Smallstep.initial_state := sys_c_initial_state se;
+          Smallstep.at_external := sys_c_at_external;
+          Smallstep.after_external := sys_c_after_external;
+          Smallstep.final_state := sys_c_final_state;
+          Smallstep.globalenv := Genv.globalenv se prog;
+        |};
+      skel := sk;
+      footprint i := False
+    |}.
+
+End SYS.
+
+Section SYS_ASM.
+  Context (prog: Asm.program).
+  Let sk := erase_program prog.
+  Section WITH_SE.
+    Context (se: Genv.symtbl).
+    Let ge := Genv.globalenv se prog.
+
+    Definition read_asm : fundef := AST.External (EF_external "read_asm" rw_sig).
+    Definition write_asm : fundef := AST.External (EF_external "write_asm" rw_sig).
+    Inductive sys_asm_initial_state: query li_asm -> sys_state -> Prop :=
+    | sys_asm_initial_state_read m n b ofs rs:
+      Genv.find_funct ge rs#PC = Some read_asm ->
+      rs#RDI = Vint (Int.repr 0) ->
+      rs#RSI = Vptr b ofs ->
+      rs#RDX = Vlong n ->
+      sys_asm_initial_state (rs, m) (sys_read_query n b ofs m)
+    | sys_asm_initial_state_write m bytes bytes_val b ofs n rs:
+      Genv.find_funct ge rs#PC = Some write_asm ->
+      rs#RDI = Vint (Int.repr 1) ->
+      rs#RSI = Vptr b ofs ->
+      rs#RDX = Vlong n ->
+      Mem.loadbytes m b (Ptrofs.unsigned ofs) (Int64.unsigned n) = Some bytes_val ->
+      map Byte bytes = bytes_val ->
+      sys_asm_initial_state (rs, m) (sys_write_query bytes m).
+
+    Inductive sys_asm_at_external: sys_state -> query (li_sys + li_sys) -> Prop :=
+    | sys_asm_at_external_read n b ofs m:
+      sys_asm_at_external (sys_read_query n b ofs m) (inl (read_query n))
+    | sys_asm_at_external_write bytes m:
+      sys_asm_at_external (sys_write_query bytes m) (inr (write_query bytes)).
+
+    Inductive sys_asm_after_external: sys_state -> reply (li_sys + li_sys) -> sys_state -> Prop :=
+    | sys_asm_after_external_read n b ofs m bytes:
+      Z.of_nat (length bytes) <= Int64.unsigned n ->
+      sys_asm_after_external (sys_read_query n b ofs m) (inl (read_reply bytes)) (sys_read_reply bytes b ofs m)
+    | sys_asm_after_external_write n m bytes:
+      sys_asm_after_external (sys_write_query bytes m) (inr (write_reply n)) (sys_write_reply n m).
+
+    Inductive sys_asm_final_state: sys_state -> reply li_asm -> Prop :=
+    | sys_asm_final_state_read bytes b ofs bytes_val m len m' (rs: regset):
+      len = Z.of_nat (length bytes) ->
+      Mem.storebytes m b (Ptrofs.unsigned ofs) bytes_val = Some m' ->
+      map Byte bytes = bytes_val ->
+      rs#RAX = Vint (Int.repr len) ->
+      sys_asm_final_state (sys_read_reply bytes b ofs m) (rs, m')
+    | sys_asm_final_state_write n m (rs: regset):
+      rs#RAX = Vint n ->
+      sys_asm_final_state (sys_write_reply n m) (rs, m).
+
+  End WITH_SE.
+  Definition sys_asm: Smallstep.semantics (li_sys + li_sys) li_asm :=
+    {|
+      activate se :=
+        {|
+          Smallstep.step _ _ _ _ := False;
+          Smallstep.initial_state := sys_asm_initial_state se;
+          Smallstep.at_external := sys_asm_at_external;
+          Smallstep.after_external := sys_asm_after_external;
+          Smallstep.final_state := sys_asm_final_state;
+          Smallstep.globalenv := Genv.globalenv se prog;
+        |};
+      skel := sk;
+      footprint i := False
+    |}.
+
+End SYS_ASM.
+
+Section SYS_C_ASM.
+
+  Local Transparent Archi.ptr64.
+
+  Lemma sys_c_asm p tp:
+    match_prog p tp -> forward_simulation 1 cc_compcert (sys_c p) (sys_asm tp).
+  Proof.
+    intros H. assert (Hsk: erase_program p = erase_program tp).
+    { apply clight_semantic_preservation in H as [H1 ?].
+      apply H1. }
+    constructor. econstructor. apply Hsk.
+    intros. reflexivity.
+    intros. instantiate (1 := fun _ _ _ => _). cbn beta.
+    eapply forward_simulation_step with (match_states := eq).
+    - intros. inv H3.
+      + unfold cc_compcert in *. cbn in wB, H2 |- *.
+        eprod_crush. destruct s9. inv H3.
+  Admitted.
+
+End SYS_C_ASM.
+
+Require Import CategoricalComp.
+
+Definition load_c (prog: Clight.program) : Smallstep.semantics (li_sys + li_sys) li_wp :=
+  let sk := AST.erase_program prog in
+  comp_semantics' (init_c prog)
+    (comp_semantics' (semantics1 prog) (sys_c prog) sk) sk.
