process/With.v
@@ -1,0 +1,81 @@
+Require Import LanguageInterface Smallstep Globalenvs Events.
+Require Import List.
+Import ListNotations.
+
+Definition empty_skel: AST.program unit unit :=
+  {|
+    AST.prog_defs := [];
+    AST.prog_public := [];
+    AST.prog_main := None;
+  |}.
+
+
+Definition with_ (liA liB: language_interface): language_interface :=
+  {|
+    query := sum (query liA) (query liB);
+    reply := sum (reply liA) (reply liB);
+    entry := fun q => match q with
+                  | inl qA => entry qA
+                  | inr qB => entry qB
+                  end;
+  |}.
+Infix "+" := with_ (at level 50, left associativity).
+
+Section WITH.
+  Context {liA1 liA2 liB1 liB2}
+    (L1: semantics liA1 liB1) (L2: semantics liA2 liB2).
+  Section WITH_SE.
+    Context (se: Genv.symtbl).
+    Definition with_state := (Smallstep.state L1 + Smallstep.state L2)%type.
+    Inductive with_initial_state: query (liB1 + liB2) -> with_state -> Prop :=
+    | with_initial_state1 q s:
+      Smallstep.initial_state (L1 se) q s ->
+      with_initial_state (inl q) (inl s)
+    | with_initial_state2 q s:
+      Smallstep.initial_state (L2 se) q s ->
+      with_initial_state (inr q) (inr s).
+    Inductive with_at_external: with_state -> query (liA1 + liA2) -> Prop :=
+    | with_at_external1 s q:
+      Smallstep.at_external (L1 se) s q ->
+      with_at_external (inl s) (inl q)
+    | with_at_external2 s q:
+      Smallstep.at_external (L2 se) s q ->
+      with_at_external (inr s) (inr q).
+    Inductive with_after_external: with_state -> reply (liA1 + liA2) -> with_state -> Prop :=
+    | with_after_external1 s r s':
+      Smallstep.after_external (L1 se) s r s' ->
+      with_after_external (inl s) (inl r) (inl s')
+    | with_after_external2 s r s':
+      Smallstep.after_external (L2 se) s r s' ->
+      with_after_external (inr s) (inr r) (inr s').
+    Inductive with_final_state: with_state -> reply (liB1 + liB2) -> Prop :=
+    | with_final_state1 s r:
+      Smallstep.final_state (L1 se) s r ->
+      with_final_state (inl s) (inl r)
+    | with_final_state2 s r:
+      Smallstep.final_state (L2 se) s r ->
+      with_final_state (inr s) (inr r).
+    Inductive with_step: with_state -> trace -> with_state -> Prop :=
+    | with_step1 s1 s1' t:
+      Step (L1 se) s1 t s1' -> with_step (inl s1) t (inl s1')
+    | with_step2 s2 s2' t:
+      Step (L2 se) s2 t s2' -> with_step (inr s2) t (inr s2').
+
+  End WITH_SE.
+
+  Definition with_semantics: semantics (liA1 + liA2) (liB1 + liB2) :=
+    {|
+      activate se :=
+        {|
+          Smallstep.step := with_step;
+          Smallstep.initial_state := with_initial_state se;
+          Smallstep.at_external := with_at_external se;
+          Smallstep.after_external := with_after_external se;
+          Smallstep.final_state := with_final_state se;
+          Smallstep.globalenv := se;
+        |};
+      skel := empty_skel;
+      footprint i := False;
+    |}.
+
+End WITH.
